Weidenbach_Book/IsaSAT/IsaSAT_Profile.thy
@@ -1,0 +1,40 @@
+theory IsaSAT_Profile
+  imports IsaSAT_Literals
+begin
+
+chapter \<open>Profiling\<close>
+
+text \<open>For profiling, we don't do anything except calling some C functions to measure time. As for
+printing, the functions to nothing in the refinement and are only removed from the generated code.
+The aim is to better understand the behaviour of the generated code and find performance bug.
+\<close>
+context
+begin
+  qualified definition start :: \<open>8 word \<Rightarrow> unit\<close> where \<open>start a = ()\<close>
+  qualified definition stop :: \<open>8 word \<Rightarrow> unit\<close> where \<open>stop a = ()\<close>
+  qualified definition PROPAGATE :: \<open>8 word\<close> where \<open>PROPAGATE = 0\<close>
+  qualified definition ANALYZE :: \<open>8 word\<close> where \<open>ANALYZE = 1\<close>
+  qualified definition GC :: \<open>8 word\<close> where \<open>GC = 2\<close>
+  qualified definition REDUCE :: \<open>8 word\<close> where \<open>REDUCE = 8\<close>
+
+qualified abbreviation start_propagate :: \<open>unit\<close> where
+  \<open>start_propagate \<equiv> IsaSAT_Profile.start IsaSAT_Profile.PROPAGATE\<close>
+qualified abbreviation stop_propagate :: \<open>unit\<close> where
+  \<open>stop_propagate \<equiv> IsaSAT_Profile.stop IsaSAT_Profile.PROPAGATE\<close>
+  qualified abbreviation start_analyze :: \<open>unit\<close> where
+  \<open>start_analyze \<equiv> IsaSAT_Profile.start IsaSAT_Profile.ANALYZE\<close>
+  qualified abbreviation stop_analyze :: \<open>unit\<close> where
+  \<open>stop_analyze \<equiv> IsaSAT_Profile.stop IsaSAT_Profile.ANALYZE\<close>
+qualified abbreviation start_GC :: \<open>unit\<close> where
+  \<open>start_GC \<equiv> IsaSAT_Profile.start IsaSAT_Profile.GC\<close>
+qualified abbreviation stop_GC :: \<open>unit\<close> where
+  \<open>stop_GC \<equiv> IsaSAT_Profile.stop IsaSAT_Profile.GC\<close>
+
+qualified abbreviation start_reduce :: \<open>unit\<close> where
+  \<open>start_reduce \<equiv> IsaSAT_Profile.start IsaSAT_Profile.REDUCE\<close>
+qualified abbreviation stop_reduce :: \<open>unit\<close> where
+  \<open>stop_reduce \<equiv> IsaSAT_Profile.stop IsaSAT_Profile.REDUCE\<close>
+
+end
+
+end
