Weidenbach_Book/IsaSAT/IsaSAT_Profile_LLVM.thy
@@ -1,0 +1,61 @@
+theory IsaSAT_Profile_LLVM
+  imports IsaSAT_Profile IsaSAT_Literals_LLVM
+begin
+
+sepref_register IsaSAT_Profile.start
+  IsaSAT_Profile.stop
+  IsaSAT_Profile.PROPAGATE
+  IsaSAT_Profile.ANALYZE
+  IsaSAT_Profile.GC
+  IsaSAT_Profile.REDUCE
+
+sepref_def start_profile
+  is \<open>RETURN o IsaSAT_Profile.start\<close>
+  :: \<open>word_assn\<^sup>k \<rightarrow>\<^sub>a unit_assn\<close>
+  unfolding IsaSAT_Profile.start_def
+  by sepref
+
+sepref_def stop_profile
+  is \<open>RETURN o IsaSAT_Profile.stop\<close>
+  :: \<open>word_assn\<^sup>k \<rightarrow>\<^sub>a unit_assn\<close>
+  unfolding IsaSAT_Profile.stop_def
+  by sepref
+
+
+sepref_def IsaSAT_Profile_PROPAGATE
+  is \<open>uncurry0 (RETURN IsaSAT_Profile.PROPAGATE)\<close>
+  :: \<open>unit_assn\<^sup>k \<rightarrow>\<^sub>a word_assn\<close>
+  unfolding IsaSAT_Profile.PROPAGATE_def
+  by sepref
+
+sepref_def IsaSAT_Profile_ANALYZE
+  is \<open>uncurry0 (RETURN IsaSAT_Profile.ANALYZE)\<close>
+  :: \<open>unit_assn\<^sup>k \<rightarrow>\<^sub>a word_assn\<close>
+  unfolding IsaSAT_Profile.ANALYZE_def
+  by sepref
+
+sepref_def IsaSAT_Profile_GC
+  is \<open>uncurry0 (RETURN IsaSAT_Profile.GC)\<close>
+  :: \<open>unit_assn\<^sup>k \<rightarrow>\<^sub>a word_assn\<close>
+  unfolding IsaSAT_Profile.GC_def
+  by sepref
+
+sepref_def IsaSAT_Profile_REDUCE
+  is \<open>uncurry0 (RETURN IsaSAT_Profile.REDUCE)\<close>
+  :: \<open>unit_assn\<^sup>k \<rightarrow>\<^sub>a word_assn\<close>
+  unfolding IsaSAT_Profile.REDUCE_def
+  by sepref
+
+
+experiment begin
+
+export_llvm
+    IsaSAT_Profile_PROPAGATE is \<open>PROFILE_CST IsaSAT_Profile_PROPAGATE\<close>
+    IsaSAT_Profile_REDUCE is \<open>PROFILE_CST IsaSAT_Profile_REDUCE\<close>
+    IsaSAT_Profile_GC is \<open>PROFILE_CST IsaSAT_Profile_GC\<close>
+    IsaSAT_Profile_ANALYZE is \<open>PROFILE_CST IsaSAT_Profile_ANALYZE\<close>
+    defines \<open>
+       typedef int8_t PROFILE_CST;
+  \<close>
+end
+end
